Orderedtree/DOrderedTree/Internal/Model.lean
@@ -1,0 +1,238 @@
+/-
+Copyright (c) 2024 Lean FRO, LLC. All rights reserved.
+Released under Apache 2.0 license as described in the file LICENSE.
+Authors: Markus Himmel
+-/
+import Orderedtree.DOrderedTree.Internal.Impl
+
+/-!
+# Model implementations of ordered tree functions
+-/
+
+set_option autoImplicit false
+set_option linter.all true
+
+universe u v w
+
+variable {α : Type u} {β : α → Type v} {γ : α → Type w} {δ : Type w}
+
+namespace Std.DOrderedTree.Internal
+
+namespace Impl
+
+/-- General "query the value at a given key" function. -/
+def queryAtKey [Ord α] (k : α) (f : Option ((a : α) × β a) → δ) (l : Impl α β) : δ :=
+  match l with
+  | .leaf => f none
+  | .inner _ k' v' l r =>
+    match compare k k' with
+    | .lt => queryAtKey k f l
+    | .eq => f (some ⟨k', v'⟩)
+    | .gt => queryAtKey k f r
+
+/-- General "update the mapping for a given key" function. -/
+def updateAtKey [Ord α] (k : α) (f : Option ((a : α) × β a) → Option ((a : α) × β a)) :
+    Impl α β → Impl α β
+| leaf => match f none with
+          | none => .leaf
+          | some ⟨k', v'⟩ => .inner 1 k' v' .leaf .leaf
+| inner sz ky y l r =>
+  match compare k ky with
+  | .lt =>
+      let newL := updateAtKey k f l
+      balanceSlow ky y newL r
+  | .eq => match f (some ⟨ky, y⟩) with
+           | none => glueSlow l r
+           | some ⟨ky', y'⟩ => .inner sz ky' y' l r
+  | .gt =>
+      let newR := updateAtKey k f r
+      balanceSlow ky y l newR
+
+/-- Model implementation of the `contains` function. -/
+def containsₘ [Ord α] (k : α) (l : Impl α β) : Bool :=
+  queryAtKey k Option.isSome l
+
+/-- Model implementation of the `insert` function. -/
+def insertₘ [Ord α] (k : α) (v : β k) (l : Impl α β) : Impl α β :=
+  updateAtKey k (fun _ => some ⟨k, v⟩) l
+
+theorem contains_eq_containsₘ [Ord α] (k : α) (l : Impl α β) :
+    l.contains k = l.containsₘ k := by
+  induction l using Impl.contains.induct k <;> simp_all [contains, containsₘ, queryAtKey]
+
+theorem balanceR_eq_balance' {k : α} {v : β k} {l r : Impl α β} {hlb hrb hlr hlr'} :
+    balanceR k v l r hlb hrb hlr = balance k v l r hlb hrb hlr' := by
+  rw [balanceR.eq_def, balance.eq_def]
+  split
+  · dsimp only
+    split
+    all_goals dsimp only
+    contradiction
+  · dsimp only
+    split
+    · dsimp only
+      split
+      all_goals try (exfalso; tree_tac)
+      congr
+      tree_tac
+    · dsimp only
+      split
+      · split
+        · dsimp only
+        · contradiction
+        · contradiction
+      · split
+        · split
+          · split
+            · exfalso; tree_tac
+            · exfalso; tree_tac
+          · contradiction
+          · contradiction
+        · rfl
+
+theorem balanceR_eq_balance {k : α} {v : β k} {l r : Impl α β} {hlb hrb hlr} :
+    balanceR k v l r hlb hrb hlr = balance k v l r hlb hrb (by tree_tac) :=
+  balanceR_eq_balance'
+
+-- This needs to be improved to balanceL_eq_balanceLErase and balanceLErase_eq_balance
+
+theorem balanceL_eq_balance' {k : α} {v : β k} {l r : Impl α β} {hlb hrb hlr hlr'} :
+    balanceL k v l r hlb hrb hlr = balance k v l r hlb hrb hlr' := by
+  rw [balanceL.eq_def, balance.eq_def]
+  split
+  · dsimp only
+    split
+    all_goals dsimp only
+    contradiction
+  · dsimp only
+    split
+    · dsimp only
+      split
+      all_goals try (exfalso; tree_tac)
+      congr
+      tree_tac
+    · dsimp only
+      split
+      · split
+        · split
+          · rename_i h
+            split
+            · exfalso; tree_tac
+            · simp [h]
+          · rename_i h
+            split
+            · exfalso; tree_tac
+            · simp [h]
+        · contradiction
+        · contradiction
+      · split
+        · exfalso; tree_tac
+        · rfl
+
+theorem balanceL_eq_balance {k : α} {v : β k} {l r : Impl α β} {hlb hrb hlr} :
+    balanceL k v l r hlb hrb hlr = balance k v l r hlb hrb (by tree_tac) :=
+  balanceL_eq_balance'
+
+theorem balanceL_eq_balanceLSlow {k : α} {v : β k} {l r : Impl α β} {hlb hrb hlr} :
+    balanceL k v l r hlb hrb hlr = balanceLSlow k v l r := by
+  rw [balanceL.eq_def, balanceLSlow.eq_def]
+  repeat' (split; dsimp)
+  all_goals try contradiction
+  all_goals simp_all [-Nat.not_lt]
+
+theorem balanceLErase_eq_balanceLSlow {k : α} {v : β k} {l r : Impl α β} {hlb hrb hlr} :
+    balanceLErase k v l r hlb hrb hlr = balanceLSlow k v l r := by
+  rw [balanceLErase.eq_def, balanceLSlow.eq_def]
+  repeat' (split; dsimp)
+  all_goals try contradiction
+  all_goals simp_all [-Nat.not_lt]
+
+theorem balanceR_eq_balanceRSlow {k : α} {v : β k} {l r : Impl α β} {hlb hrb hlr} :
+    balanceR k v l r hlb hrb hlr = balanceRSlow k v l r := by
+  rw [balanceR.eq_def, balanceRSlow.eq_def]
+  repeat' (split; dsimp)
+  all_goals try contradiction
+  all_goals simp_all [-Nat.not_lt]
+
+theorem balanceRErase_eq_balanceRSlow {k : α} {v : β k} {l r : Impl α β} {hlb hrb hlr} :
+    balanceRErase k v l r hlb hrb hlr = balanceRSlow k v l r := by
+  rw [balanceRErase.eq_def, balanceRSlow.eq_def]
+  repeat' (split; dsimp)
+  all_goals try contradiction
+  all_goals simp_all [-Nat.not_lt]
+
+theorem balance_eq_balanceSlow {k : α} {v : β k} {l r : Impl α β} {hlb hrb hlr} :
+    balance k v l r hlb hrb hlr = balanceSlow k v l r := by
+  rw [balance.eq_def, balanceSlow.eq_def]
+  repeat' (split; dsimp)
+  all_goals try contradiction
+  all_goals simp_all [-Nat.not_lt]
+
+theorem minView_k_eq_minViewSlow {k : α} {v : β k} {l r : Impl α β} {hl hr hlr} :
+    (minView k v l r hl hr hlr).k = (minViewSlow k v l r).k := by
+  induction k, v, l, r, hl, hr, hlr using minView.induct <;> simp_all [minView, minViewSlow]
+
+theorem minView_kv_eq_minViewSlow {k : α} {v : β k} {l r : Impl α β} {hl hr hlr} :
+    (⟨(minView k v l r hl hr hlr).k, (minView k v l r hl hr hlr).v⟩ : (a : α) × β a) =
+      ⟨(minViewSlow k v l r).k, (minViewSlow k v l r).v⟩ := by
+  induction k, v, l, r, hl, hr, hlr using minView.induct <;>
+    simp_all [minView, minViewSlow]
+
+theorem minView_tree_impl_eq_minViewSlow {k : α} {v : β k} {l r : Impl α β} {hl hr hlr} :
+    (minView k v l r hl hr hlr).tree.impl = (minViewSlow k v l r).tree := by
+  induction k, v, l, r, hl, hr, hlr using minView.induct <;>
+    simp_all [minView, minViewSlow, balanceRErase_eq_balanceRSlow]
+
+theorem maxView_k_eq_maxViewSlow {k : α} {v : β k} {l r : Impl α β} {hl hr hlr} :
+    (maxView k v l r hl hr hlr).k = (maxViewSlow k v l r).k := by
+  induction k, v, l, r, hl, hr, hlr using maxView.induct <;> simp_all [maxView, maxViewSlow]
+
+theorem maxView_kv_eq_maxViewSlow {k : α} {v : β k} {l r : Impl α β} {hl hr hlr} :
+    (⟨(maxView k v l r hl hr hlr).k, (maxView k v l r hl hr hlr).v⟩ : (a : α) × β a) =
+      ⟨(maxViewSlow k v l r).k, (maxViewSlow k v l r).v⟩ := by
+  induction k, v, l, r, hl, hr, hlr using maxView.induct <;>
+    simp_all [maxView, maxViewSlow]
+
+theorem maxView_tree_impl_eq_maxViewSlow {k : α} {v : β k} {l r : Impl α β} {hl hr hlr} :
+    (maxView k v l r hl hr hlr).tree.impl = (maxViewSlow k v l r).tree := by
+  induction k, v, l, r, hl, hr, hlr using maxView.induct <;>
+    simp_all [maxView, maxViewSlow, balanceLErase_eq_balanceLSlow]
+
+theorem balanceLSlow_pair_congr {k : α} {v : β k} {k' : α} {v' : β k'}
+    (h : (⟨k, v⟩ : (a : α) × β a) = ⟨k', v'⟩) {l l' r r' : Impl α β}
+    (hl : l = l') (hr : r = r') :
+    balanceLSlow k v l r = balanceLSlow k' v' l' r' := by
+  cases h; cases hl; cases hr; rfl
+
+theorem balanceRSlow_pair_congr {k : α} {v : β k} {k' : α} {v' : β k'}
+    (h : (⟨k, v⟩ : (a : α) × β a) = ⟨k', v'⟩) {l l' r r' : Impl α β}
+    (hl : l = l') (hr : r = r') :
+    balanceRSlow k v l r = balanceRSlow k' v' l' r' := by
+  cases h; cases hl; cases hr; rfl
+
+theorem glue_eq_glueSlow {l r : Impl α β} {hl hr hlr} :
+    glue l r hl hr hlr = glueSlow l r := by
+  rw [glue.eq_def, glueSlow.eq_def]
+  split; simp
+  split; simp
+  dsimp only
+  split
+  · simpa [*, balanceLErase_eq_balanceLSlow] using balanceLSlow_pair_congr
+      minView_kv_eq_minViewSlow rfl minView_tree_impl_eq_minViewSlow
+  · simpa [*, balanceRErase_eq_balanceRSlow] using balanceRSlow_pair_congr
+      maxView_kv_eq_maxViewSlow maxView_tree_impl_eq_maxViewSlow rfl
+
+theorem insert_eq_insertSlow [Ord α] {k : α} {v : β k} {l : Impl α β} {h} :
+    (insert k v l h).impl = insertSlow k v l := by
+  induction l, h using insert.induct k v <;>
+    simp_all [insert, insertSlow, balanceL_eq_balanceLSlow, balanceR_eq_balanceRSlow]
+
+theorem insert_eq_insertₘ [Ord α] {k : α} {v : β k} {l : Impl α β} {h} :
+    (insert k v l h).impl = insertₘ k v l := by
+  induction l, h using insert.induct k v <;>
+    simp_all [insert, insertₘ, updateAtKey, balanceL_eq_balance, balanceR_eq_balance,
+      balance_eq_balanceSlow]
+
+end Impl
+
+end Std.DOrderedTree.Internal
