Orderedtree/DOrderedTree/Internal/WF.lean
@@ -1,0 +1,23 @@
+/-
+Copyright (c) 2024 Lean FRO, LLC. All rights reserved.
+Released under Apache 2.0 license as described in the file LICENSE.
+Authors: Markus Himmel
+-/
+import Orderedtree.DOrderedTree.Internal.Impl
+
+/-!
+# Low-level proofs about size-bounded trees
+-/
+
+set_option autoImplicit false
+set_option linter.all true
+
+universe u v w
+
+variable {α : Type u} {β : α → Type v} {γ : α → Type w} {δ : Type v}
+
+namespace Std.DOrderedTree.Internal
+
+
+
+end Std.DOrderedTree.Internal
